Compiles UFSource

demo/union_find/UnionFindSource.v
@@ -9,54 +9,39 @@ Require ClightC.
 Require Import UnionFindTarget.
 Require Import SIR.
 
+(* Require Import Clightdefs. *)
+
 From ExtLib Require Import
      OptionMonad
      Functor FunctorLaws
+     Structures.Maps
 .
-Import FunctorNotation.
 
 Set Implicit Arguments.
 
+
+Import FunctorNotation.
+Local Open Scope monad_scope.
+Notation "` x : t <- t1 ;; t2" := (ITree.bind t1 (fun x : t => t2))
+  (at level 61, t at next level, t1 at next level, x ident, right associativity) : itree_scope.
+
+
 Local Obligation Tactic := ii; ss; des; inv_all_once; repeat des_u; ss; clarify.
 
-Definition update V (map: block -> option V) (k0: block) (v: option V): block -> option V :=
-  fun k1 => if eq_block k0 k1 then v else map k1.
+Program Instance function_MapOk (K V: Type) (dec: forall k0 k1, {k0=k1} + {k0<>k1}):
+  MapOk eq (function_Map V dec) (K := K) := {| mapsto := fun k v m => m k = Some v |}.
+Next Obligation. des_ifs. Qed.
+Next Obligation. des_ifs. Qed.
+Next Obligation. des_ifs. Qed.
+Next Obligation. des_ifs. Qed.
 
-Definition owned_heap: Type := block -> option (block * int).
-Definition initial_owned_heap: SkEnv.t -> owned_heap := fun _ => fun _ => None.
-
-Variable global_definitions:
-  list (ident * globdef (fundef (SIR.function owned_heap)) unit).
-
-Definition c_makeSet (vs: list val): itree (E owned_heap) val :=
-  m0 <- trigger (Get _) ;; oh0 <- trigger (Get _) ;;
-  let '(m1, blk) := (Mem.alloc m0 0%Z 0%Z) in
-  let oh1 := update oh0 blk (Some (blk, Int.zero)) in
-  trigger (Put _ m1) ;; trigger (Put _ oh1) ;;
-  Ret (Vptr blk Ptrofs.zero)
-.
-
-Definition c_makeSet_old (oh0: owned_heap) (vs: list val) (m0: mem):
-  itree (E owned_heap) (owned_heap * mem * val) :=
-  let '(m1, blk) := (Mem.alloc m0 0%Z 0%Z) in
-  let oh1 := update oh0 blk (Some (blk, Int.zero)) in
-  Ret (oh1, m1, (Vptr blk Ptrofs.zero))
-.
-
-Definition f_makeSet: function owned_heap :=
-  mkfunction (ClightC.signature_of_function f_makeSet) c_makeSet.
-
-Definition g_makeSet:
-  (ident * globdef (fundef (SIR.function owned_heap)) unit) :=
-  (_makeSet, Gfun(Internal f_makeSet)).
-
-Definition assume (P: Prop): itree (E owned_heap) unit :=
+Definition assume oh (P: Prop): itree (E oh) unit :=
   if ClassicalDescription.excluded_middle_informative P
   then Ret tt
   else triggerUB "assume"
 .
   
-Definition guarantee (P: Prop): itree (E owned_heap) unit :=
+Definition guarantee oh (P: Prop): itree (E oh) unit :=
   if ClassicalDescription.excluded_middle_informative P
   then Ret tt
   else triggerNB "guarantee"
@@ -72,350 +57,82 @@ Definition unblock (v: val): option block :=
   end
 .
 
-Local Open Scope monad_scope.
 
-Definition c_find (vs: list val):
-  itree (E owned_heap) val :=
+
+
+Definition owned_heap: Type := block -> option (block * int).
+Instance owned_heap_Map: (Map _ _ owned_heap) := function_Map _ eq_block.
+Definition initial_owned_heap: SkEnv.t -> owned_heap := fun _ => Maps.empty.
+
+Definition c_makeSet (vs: list val): itree (E owned_heap) val :=
+  m0 <- trigger (Get _) ;; oh0 <- trigger (Get _) ;;
+  let '(m1, blk) := (Mem.alloc m0 0%Z 0%Z) in
+  let oh1: owned_heap := Maps.add blk (blk, Int.zero) oh0 in
+  trigger (Put _ m1) ;; trigger (Put _ oh1) ;;
+  Ret (Vptr blk Ptrofs.zero)
+.
+
+Definition c_makeSet_old (oh0: owned_heap) (vs: list val) (m0: mem):
+  itree (E owned_heap) (owned_heap * mem * val) :=
+  let '(m1, blk) := (Mem.alloc m0 0%Z 0%Z) in
+  let oh1 := Maps.add blk (blk, Int.zero) oh0 in
+  Ret (oh1, m1, (Vptr blk Ptrofs.zero))
+.
+
+Definition f_makeSet: function owned_heap :=
+  mkfunction (ClightC.signature_of_function f_makeSet) c_makeSet.
+
+Definition c_find (vs: list val): itree (E owned_heap) val :=
   oh0 <- trigger (Get _) ;;
   x <- unwrapU ((hd_error vs) >>= unblock) ;;
-  '(p, _) <- unwrapU (oh0 x) ;;
-  if negb (eq_block p x)
-  (* then (p0 <- trigger (ICall _find [Vptr p Ptrofs.zero]) ;; *)
-  (*          p0 <- unwrapN (unblock p0);; *)
-  (*         triggerUB "") *)
-  then p0 <- (unblock <$> (trigger (ICall _find [Vptr p Ptrofs.zero])) >>= unwrapN) ;;
-          triggerUB ""
-  else triggerUB ""
-  (* x <- (@bind option Monad_option _ _ (hd_error vs) unblock) ;; *)
-  (* triggerUB "" *)
-.
-Variable E: Type -> Type.
-Variable R: Type.
-Definition trans `{EventE -< E} (itr: itree E (option R)): (itree E R) :=
-  (* r <- itr ;; r <- unwrapN r ;; Ret r *)
-  itr >>= unwrapN
-.
-  
-Variable itr: itree E (option R).
-Definition itr2: option (itree E R).
-MonadIter_optionT
-optionT
-
-  if (p != x) {
-    p0 = find(p);
-    x -> parent = p0;
-  }
-  return p;
-
-Definition c_find (oh0: owned_heap) (vs: list val) (m0: mem):
-  itree (eff owned_heap) (owned_heap * mem * val) :=
-  match vs with
-  | [Vptr x ofs] =>
-    assume (Ptrofs.eq_dec ofs Ptrofs.zero) ;;
-    '(p, rx) <- unwrapU (oh0 blk) ;;
-    if negb (block_eq p x)
-    then
-      p0 <- trigger (ICall _find oh0 ([Vptr p Ptrofs.zero]) m0) ;;
-      match p0 with
-      | [Vptr p0 ofs] =>
-        guarantee (Ptrofs.eq_dec ofs Ptrofs.zero) ;;
-        let oh1 := update oh0 x (Some (p0, rx)) in
-        Ret tt
-    else Ret tt;;
-    Ret (
-  | _ => triggerUB ""
-  end
+  '(p, rk) <- unwrapU (Maps.lookup x oh0) ;; trigger (LPut _p (Vptr p Ptrofs.zero)) ;;
+  (if negb (eq_block p x)
+   then `p0: block <- (unblock <$> (trigger (ICall _find [Vptr p Ptrofs.zero])) >>= unwrapN) ;;
+        trigger (LPut _p (Vptr p0 Ptrofs.zero)) ;;
+        let oh1 := Maps.add x (p0, rk) oh0 in
+        trigger (Put _ oh1)
+   else Ret tt) ;;
+  trigger (LGet _p) >>= ret
 .
 
-struct Node* find(struct Node* x) {
-  struct Node *p, *p0;
-  p = x -> parent;
-  if (p != x) {
-    p0 = find(p);
-    x -> parent = p0;
-  }
-  return p;
-};
+Definition f_find: function owned_heap :=
+  mkfunction (ClightC.signature_of_function f_find) c_find.
 
-void unionS(struct Node* x, struct Node* y) {
-  struct Node *xRoot, *yRoot;
-  unsigned int xRank, yRank;
-  xRoot = find(x);
-  yRoot = find(y);
-  if (xRoot == yRoot) {
-    return;
-  }
-  xRank = xRoot -> rank;
-  yRank = yRoot -> rank;
-  if (xRank < yRank) {
-    xRoot -> parent = yRoot;
-  } else if (xRank > yRank) {
-    yRoot -> parent = xRoot;
-  } else {
-    yRoot -> parent = xRoot;
-    xRoot -> rank = xRank + 1;
-  }
-};
+Definition global_definitions: list (ident * globdef (fundef (SIR.function owned_heap)) unit) :=
+((_malloc, Gfun(External EF_malloc)) ::
+ (_makeSet, Gfun(Internal f_makeSet)) :: (_find, Gfun(Internal f_find)) ::
+ (* (_unionS, Gfun(Internal f_unionS)) :: *)
+ (* (_same_set, Gfun(Internal f_same_set)) :: *)
+ nil
+)
+.
 
-/////////////////////////////////////////////////
+Definition prog: SIR.program owned_heap := mkprogram global_definitions public_idents _main.
 
-int same_set(struct Node* x, struct Node *y) {
-  return (find(x) == find(y));
-}
+Definition module: Mod.t := SIR.module prog "UF"%string initial_owned_heap.
 
+(* void unionS(struct Node* x, struct Node* y) { *)
+(*   struct Node *xRoot, *yRoot; *)
+(*   unsigned int xRank, yRank; *)
+(*   xRoot = find(x); *)
+(*   yRoot = find(y); *)
+(*   if (xRoot == yRoot) { *)
+(*     return; *)
+(*   } *)
+(*   xRank = xRoot -> rank; *)
+(*   yRank = yRoot -> rank; *)
+(*   if (xRank < yRank) { *)
+(*     xRoot -> parent = yRoot; *)
+(*   } else if (xRank > yRank) { *)
+(*     yRoot -> parent = xRoot; *)
+(*   } else { *)
+(*     yRoot -> parent = xRoot; *)
+(*     xRoot -> rank = xRank + 1; *)
+(*   } *)
+(* }; *)
 
-Definition prog: SIR.program owned_heap :=
-  mkprogram global_definitions public_idents _main.
+(* ///////////////////////////////////////////////// *)
 
-Variable p: program owned_heap.
-Definition module: Mod.t := SIR.module p "UF" (initial_owned_heap).
-
-
-(_makeSet, Gfun(Internal f_makeSet)) :: (_find, Gfun(Internal f_find)) ::
- (_unionS, Gfun(Internal f_unionS)) ::
- (_same_set, Gfun(Internal f_same_set))
-
-
-
-
-
-
-
-
-
-
-Section MODSEM.
-
-  Variable skenv_link: SkEnv.t.
-  Let skenv: SkEnv.t := (SkEnv.project skenv_link) (CSk.of_program signature_of_function prog).
-
-  Definition owned_heap: Type := key -> option (int * bool).
-  Variable p: SIR.program owned_heap.
-  Definition initial_owned_heap: owned_heap := fun _ => None.
-
-  Inductive state: Type :=
-  | CallstateNew
-      (v: int)
-      (oh: owned_heap) (m: mem)
-  | CallstateGet
-      (k: key)
-      (oh: owned_heap) (m: mem)
-  | CallstateSet
-      (k: key)
-      (v: int)
-      (oh: owned_heap) (m: mem)
-  | CallstateDelete
-      (k: key)
-      (oh: owned_heap) (m: mem)
-  | CallstateFromRaw
-      (k: key)
-      (oh: owned_heap) (m: mem)
-  | CallstateIntoRaw
-      (k: key)
-      (oh: owned_heap) (m: mem)
-  | ReturnstateNew
-      (k: key)
-      (oh: owned_heap) (m: mem)
-  | ReturnstateGet
-      (v: int)
-      (oh: owned_heap) (m: mem)
-  | ReturnstateSet
-      (oh: owned_heap) (m: mem)
-  | ReturnstateDelete
-      (oh: owned_heap) (m: mem)
-  | ReturnstateFromRaw
-      (k: key)
-      (oh: owned_heap) (m: mem)
-  | ReturnstateIntoRaw
-      (k: key)
-      (oh: owned_heap) (m: mem)
-  .
-
-  (*** TODO:
-we can say that,
-(1) if is_raw is false (new/delete) --> ptrofs is zero
-(2) mem.valid_block thing
-   ***)
-  Definition oh_wf: owned_heap -> Prop := top1.
-
-  Inductive initial_frame (oh: owned_heap) (args: Args.t): state -> Prop :=
-  | initial_frame_new
-      (WF: oh_wf oh)
-      m blk val
-      (SYMB: Genv.find_symbol skenv _new = Some blk)
-      (FPTR: (Args.fptr args) = Vptr blk Ptrofs.zero)
-      (VS: (Args.vs args) = [Vint val])
-      (M: (Args.m args) = m)
-    :
-      initial_frame oh args (CallstateNew val oh m)
-  | initial_frame_get
-      (WF: oh_wf oh)
-      m blk key
-      (SYMB: Genv.find_symbol skenv _get = Some blk)
-      (FPTR: (Args.fptr args) = Vptr blk Ptrofs.zero)
-      (VS: (Args.vs args) = [Vptr key Ptrofs.zero])
-      (M: (Args.m args) = m)
-    :
-      initial_frame oh args (CallstateGet key oh m)
-  | initial_frame_set
-      (WF: oh_wf oh)
-      m blk key val
-      (SYMB: Genv.find_symbol skenv _get = Some blk)
-      (FPTR: (Args.fptr args) = Vptr blk Ptrofs.zero)
-      (OHSOME: oh key <> None)
-      (VS: (Args.vs args) = [Vptr key Ptrofs.zero ; Vint val])
-      (M: (Args.m args) = m)
-    :
-      initial_frame oh args (CallstateSet key val oh m)
-  | initial_frame_delete
-      (WF: oh_wf oh)
-      m blk key
-      (SYMB: Genv.find_symbol skenv _delete = Some blk)
-      (FPTR: (Args.fptr args) = Vptr blk Ptrofs.zero)
-      (VS: (Args.vs args) = [Vptr key Ptrofs.zero])
-      (M: (Args.m args) = m)
-    :
-      initial_frame oh args (CallstateDelete key oh m)
-  | initial_frame_from_raw
-      (WF: oh_wf oh)
-      m blk key
-      (SYMB: Genv.find_symbol skenv _from_raw = Some blk)
-      (FPTR: (Args.fptr args) = Vptr blk Ptrofs.zero)
-      (VS: (Args.vs args) = [Vptr key Ptrofs.zero])
-      (M: (Args.m args) = m)
-    :
-      initial_frame oh args (CallstateFromRaw key oh m)
-  | initial_frame_into_raw
-      (WF: oh_wf oh)
-      m blk key
-      (SYMB: Genv.find_symbol skenv _into_raw = Some blk)
-      (FPTR: (Args.fptr args) = Vptr blk Ptrofs.zero)
-      (VS: (Args.vs args) = [Vptr key Ptrofs.zero])
-      (M: (Args.m args) = m)
-    :
-      initial_frame oh args (CallstateIntoRaw key oh m)
-  .
-
-  Inductive step (se: Senv.t) (ge: SkEnv.t): state -> trace -> state -> Prop :=
-  | step_new
-      oh0 m0 oh1 m1 m2 key val
-      (ALLOC: Mem.alloc m0 lo hi = (m1, key))
-      (FREE: Mem.free m1 key lo hi = Some m2)
-      (OH: update oh0 key (Some (val, false)) = oh1)
-    :
-      step se ge (CallstateNew val oh0 m0) E0 (ReturnstateNew key oh1 m2)
-  | step_get
-      oh m key val is_raw
-      (GET: oh key = Some (val, is_raw))
-    :
-      step se ge (CallstateGet key oh m) E0 (ReturnstateGet val oh m)
-  | step_set
-      oh0 m key val oh1 UNUSED_oldval is_raw
-      (SOME: oh0 key = Some (UNUSED_oldval, is_raw))
-      (SET: update oh0 key (Some (val, is_raw)) = oh1)
-    :
-      step se ge (CallstateSet key val oh0 m) E0 (ReturnstateSet oh1 m)
-  | step_delete
-      oh0 m key UNUSED_oldval oh1
-      (SOME: oh0 key = Some (UNUSED_oldval, false))
-      (SET: update oh0 key None = oh1)
-    :
-      step se ge (CallstateDelete key oh0 m) E0 (ReturnstateDelete oh1 m)
-  | step_from_raw
-      oh0 m0 key val oh1 m1
-      (LOAD: Mem.load Mint32 m0 key 0%Z = Some (Vint val))
-      (FREE: Mem.free m0 key 0%Z hi = Some m1)
-      (NONE: oh0 key = None) (*** <- TODO: is it needed? ***)
-      (SET: update oh0 key (Some (val, true)) = oh1)
-    :
-      step se ge (CallstateFromRaw key oh0 m0) E0 (ReturnstateFromRaw key oh1 m1)
-  | step_into_raw
-      oh0 m0 key val m1 oh1 m2
-      (*** TODO: we should "GUARANTEE" that store succeeds. ***)
-      (SOME: oh0 key = Some (val, true))
-      (UNFREE: Mem_unfree m0 key 0%Z hi  = Some m1)
-      (STORE: Mem_stored Mint32 m1 key 0%Z (Vint val) m2)
-      (SET: update oh0 key None = oh1)
-    :
-      step se ge (CallstateIntoRaw key oh0 m0) E0 (ReturnstateIntoRaw key oh1 m2)
-  .
-
-  Inductive final_frame: state -> owned_heap -> Retv.t -> Prop :=
-  | final_new
-      key oh m
-    :
-      final_frame (ReturnstateNew key oh m) oh (Retv.mk (Vptr key Ptrofs.zero) m)
-  | final_get
-      val oh m
-    :
-      final_frame (ReturnstateGet val oh m) oh (Retv.mk (Vint val) m)
-  | final_set
-      oh m
-    :
-      final_frame (ReturnstateSet oh m) oh (Retv.mk Vundef m)
-  | final_delete
-      oh m
-    :
-      final_frame (ReturnstateDelete oh m) oh (Retv.mk Vundef m)
-  | final_from_raw
-      key oh m
-    :
-      final_frame (ReturnstateFromRaw key oh m) oh (Retv.mk (Vptr key Ptrofs.zero) m)
-  | final_into_raw
-      key oh m
-    :
-      final_frame (ReturnstateIntoRaw key oh m) oh (Retv.mk (Vptr key Ptrofs.zero) m)
-  .
-
-  Program Definition modsem: ModSem.t :=
-    {|
-      ModSem.step := step;
-      ModSem.at_external := bot3;
-      ModSem.initial_frame := initial_frame;
-      ModSem.final_frame := final_frame;
-      ModSem.after_external := bot4;
-      ModSem.globalenv := skenv;
-      ModSem.skenv := skenv;
-      ModSem.midx := Some "OHAlloc";
-      ModSem.skenv_link := skenv_link;
-      ModSem.owned_heap := owned_heap;
-      ModSem.initial_owned_heap := initial_owned_heap;
-    |}
-  .
-
-End MODSEM.
-
-Program Definition module: Mod.t :=
-  {| Mod.data := tt; Mod.get_sk := fun _ => CSk.of_program signature_of_function prog; Mod.get_modsem := modsem; Mod.midx := Some "OHAlloc" |}.
-
-(* Lemma find_symbol_find_funct_ptr *)
-(*       skenv_link blk *)
-(*       ske *)
-(*       (WF: SkEnv.wf skenv_link) *)
-(*       (INCL: SkEnv.includes skenv_link (CSk.of_program signature_of_function MutrecA.prog)) *)
-(*       (SKE: ske = (SkEnv.project skenv_link (CSk.of_program signature_of_function MutrecA.prog))) : *)
-(*     (<<SYMB: Genv.find_symbol ske f_id = Some blk>>) <-> *)
-(*     (<<FINDF: exists if_sig, Genv.find_funct_ptr ske blk = Some (AST.Internal if_sig)>>). *)
-(* Proof. *)
-(*   clarify. *)
-(*   hexploit (SkEnv.project_impl_spec INCL); eauto. intro PROJ. *)
-(*   exploit SkEnv.project_spec_preserves_wf; eauto. intro WFSMALL. *)
-(*   inv INCL. specialize (DEFS f_id). ss. exploit DEFS; eauto. i; des. *)
-(*   inv MATCH. inv H0. *)
-(*   inv PROJ. exploit (SYMBKEEP f_id); eauto. intro T; des. rewrite T in *. *)
-(*   exploit DEFKEEP; eauto. *)
-(*   { eapply Genv.find_invert_symbol; et. } *)
-(*   { ss. } *)
-(*   i; des. *)
-(*   inv LO. inv H1; ss. clarify. *)
-(*   split; ii; ss; des; clarify. *)
-(*   - unfold Genv.find_funct_ptr. rewrite DEFSMALL. ss. esplits; eauto. *)
-(*   - unfold Genv.find_funct_ptr in *. des_ifs. *)
-(*     clear_tac. *)
-(*     assert(blk = blk0). *)
-(*     { clear - DEFSMALL Heq. *)
-(*       uge. ss. rewrite MapsC.PTree_filter_map_spec in *. uo. des_ifs. *)
-(*       apply_all_once in_prog_defmap. ss. unfold update_snd in *. ss. des; clarify. *)
-(*       apply_all_once Genv.invert_find_symbol. clarify. *)
-(*     } clarify. *)
-(* Qed. *)
+(* int same_set(struct Node* x, struct Node *y) { *)
+(*   return (find(x) == find(y)); *)
+(* } *)
